

$$\begin{aligned}
 1a) \quad S(1,1) &= 47 \cdot 0 + 162 \cdot 0 + 47 \cdot 0 + 0 + 0 + 0 - 47 \cdot 0 - 162 \cdot 100 - 47 \cdot 100 = -20900 \\
 S(1,2) &= 100 \cdot 162 + 47 \cdot 100 + 0 + 0 + 0 - 100 \cdot 162 - 47 \cdot 100 \cdot 47 = -4700 \\
 S(2,1) &= 100 \cdot 47 + 0 + 0 + 0 - 47 \cdot 100 - 162 \cdot 100 - 47 \cdot 100 = -20900 \\
 S(2,2) &= 0 \\
 S(1,3) &= 0 \\
 S(2,3) &= 100 \cdot 162 + 47 \cdot 100 = 20900 \\
 S(3,1) &= 0 \\
 S(3,2) &= 4700 \\
 S(3,3) &= 20900
 \end{aligned}$$

$$\Rightarrow P_k = \begin{pmatrix} -20900 & -4700 & 0 \\ -20900 & 0 & 20900 \\ 0 & 4700 & 20900 \end{pmatrix}$$

$$P_{G_v} = \begin{pmatrix} -20900 & -20900 & 0 \\ -4700 & 0 & 4700 \\ 0 & 20900 & 20900 \end{pmatrix} \quad \text{Rechnung analog zu oben für die Werte nur mit } G_v$$

$$c) \quad S \approx \sqrt{S_x(x,y)^2 + S_y(x,y)^2}$$

$$S(1,1) = \sqrt{20900^2 + (-20900)^2} \approx 29557$$

⋮

$$S = \begin{pmatrix} 29557 & \sqrt{4700^2 + 20900^2} & 0 \\ \sqrt{20900^2 + 4700^2} & 0 & 0 \\ 0 & \sqrt{4700^2 + 20900^2} & 29557 \end{pmatrix}$$

$$d) \quad \theta \approx \begin{cases} \arctan(S_y(x,y)/S_x(x,y)) & \text{für } S_x(x,y) \neq 0 \\ 90^\circ & \text{für } S_x(x,y) = 0, S_y(x,y) \neq 0 \end{cases}$$

$$\theta = \begin{pmatrix} 45 & \nearrow \nearrow & 2 \\ 13 & ? & 13 \\ 2 & \nearrow \nearrow & 45 \end{pmatrix} \rightarrow \text{undefiniert, da } S_x(x,y) \wedge S_y(x,y) = 0 \\
 \rightarrow \text{gerundete Werte}$$

3

$$a) \frac{\partial f}{\partial x_1} = 2x_1 \quad \frac{\partial f}{\partial x_2} = 2x_2 \quad \frac{\partial f}{\partial x_3} = 2x_3$$

$$\frac{\partial^2 f}{\partial x_1^2} = 2 \quad \frac{\partial^2 f}{\partial x_2^2} = 2 \quad \frac{\partial^2 f}{\partial x_3^2} = 2$$

$$\nabla^2 f = 2 + 2 + 2 = 6$$

$$b) \frac{\partial f}{\partial x_1} = (2x_1) \cdot x_2^2 \cdot x_3$$

$$\frac{\partial f}{\partial x_2} = x_1^2 \cdot (2x_2) \cdot x_3$$

$$\frac{\partial f}{\partial x_3} = x_1^2 \cdot x_2^2 \cdot 1$$

$$\frac{\partial^2 f}{\partial x_1^2} = 2 \cdot x_2^2 \cdot x_3$$

$$\frac{\partial^2 f}{\partial x_2^2} = x_1^2 \cdot (2) \cdot x_3$$

$$\frac{\partial^2 f}{\partial x_3^2} = x_1^2 \cdot x_2^2 \cdot 0$$

$$\begin{aligned} \nabla^2 f &= 2x_2^2 \cdot x_3 + 2x_1^2 \cdot x_3 + 0 \\ &= 2x_3 (x_1^2 + x_2^2) \end{aligned}$$